Progress on translation (pat_to_clos) - The translator fix was to support mutually recursive definitions   where the name appearing in the induction theorem isn't the same as   the first name that appears in the definition   (see renumber_code_locs_ind and renumber_code_locs_list) - The minor fix might not be sufficient

compiler/backend/pat_to_closScript.sml
@@ -21,7 +21,7 @@ val compile_def = tDefine"compile"`
   (compile (Lit (Word8 w)) =
     Op (Const (& (w2n w))) []) ∧
   (compile (Lit (Word64 w)) =
-    Op WordFromInt [Op (Const (w2i w)) []]) ∧
+    Op WordFromInt [Op (Const (&(w2n w))) []]) ∧
   (compile (Lit (Char c)) =
     Op (Const (& ORD c)) []) ∧
   (compile (Lit (StrLit s)) =
